Remove fmap_of.

theories/fmap.v
@@ -73,33 +73,31 @@ Variables (T : ordType) (S : Type).
 
 Local Open Scope ord_scope.
 
-Record fmap_type := FMap {
+Record fmap_type (p : phant (T -> S)) := FMap {
   fmval : seq (T * S);
   _ : sorted (@Ord.lt T) (unzip1 fmval)
 }.
-Definition fmap_of of phant (T -> S) := fmap_type.
-Identity Coercion type_of_fmap_of : fmap_of >-> fmap_type.
 
 End Def.
 
 Module Exports.
 
-Notation "{ 'fmap' T }" := (@fmap_of _ _ (Phant T))
+Notation "{ 'fmap' T }" := (@fmap_type _ _ (Phant T))
   (at level 0, format "{ 'fmap'  T }") : type_scope.
 Coercion fmval : fmap_type >-> seq.
-Canonical fmap_subType T S := [subType for @fmval T S].
-Definition fmap_eqMixin T (S : eqType) :=
-  [eqMixin of fmap_type T S by <:].
-Canonical fmap_eqType T (S : eqType) :=
-  Eval hnf in EqType (fmap_type T S) (fmap_eqMixin T S).
-Definition fmap_choiceMixin T (S : choiceType) :=
-  [choiceMixin of fmap_type T S by <:].
-Canonical fmap_choiceType T (S : choiceType) :=
-  Eval hnf in ChoiceType (fmap_type T S) (fmap_choiceMixin T S).
-Definition fmap_ordMixin T (S : ordType) :=
-  [ordMixin of fmap_type T S by <:].
-Canonical fmap_ordType T (S : ordType) :=
-  Eval hnf in OrdType (fmap_type T S) (fmap_ordMixin T S).
+Canonical fmap_subType T S p := [subType for @fmval T S p].
+Definition fmap_eqMixin T (S : eqType) p :=
+  [eqMixin of @fmap_type T S p by <:].
+Canonical fmap_eqType T (S : eqType) p :=
+  Eval hnf in EqType (@fmap_type T S p) (@fmap_eqMixin T S p).
+Definition fmap_choiceMixin T (S : choiceType) p :=
+  [choiceMixin of @fmap_type T S p by <:].
+Canonical fmap_choiceType T (S : choiceType) p :=
+  Eval hnf in ChoiceType (@fmap_type T S p) (@fmap_choiceMixin T S p).
+Definition fmap_ordMixin T (S : ordType) p :=
+  [ordMixin of @fmap_type T S p by <:].
+Canonical fmap_ordType T (S : ordType) p :=
+  Eval hnf in OrdType (@fmap_type T S p) (@fmap_ordMixin T S p).
 
 (*
 
@@ -119,23 +117,10 @@ End FMap.
 
 Export FMap.Exports.
 
-Section ReExports.
-
-Variable T : ordType.
-Canonical fmap_of_subType S := Eval hnf in [subType of {fmap T -> S}].
-Canonical fmap_of_eqType (S : eqType) :=
-  Eval hnf in [eqType of {fmap T -> S}].
-Canonical fmap_of_choiceType (S : choiceType) :=
-  Eval hnf in [choiceType of {fmap T -> S}].
-Canonical fmap_of_ordType (S : ordType) :=
-  Eval hnf in [ordType of {fmap T -> S}].
-
-End ReExports.
-
 (* Redefine the fmap constructor with a different signature, in
 order to keep types consistent. *)
 Definition fmap (T : ordType) S s Ps : {fmap T -> S} :=
-  @FMap.FMap T S s Ps.
+  @FMap.FMap T S _ s Ps.
 
 Section Operations.
 
@@ -152,11 +137,7 @@ Fixpoint getm_def s k : option S :=
     else getm_def s k
   else None.
 
-(* It seems that we need to declare getm with fmap_type as opposed to
-   fmap_of, in order to make the coercion into Funclass below to work. The
-   finfun module in mathcomp seems to suffer from a similar issue. *)
-
-Definition getm (m : FMap.fmap_type T S) k := getm_def m k.
+Definition getm p (m : @FMap.fmap_type T S p) k := getm_def m k.
 
 Fixpoint setm_def s k v : seq (T * S) :=
   if s is p :: s' then
@@ -776,9 +757,9 @@ Definition currym m :=
                                    (@snd _ _ @: domm m))
              (@fst _ _ @: domm m).
 
-Definition uncurrym n :=
-  mkfmapfp (fun p => if n p.1 is Some n' then n' p.2
-                        else None)
+Definition uncurrym n : {fmap T * S -> R} :=
+  mkfmapfp (fun p : T * S => if n p.1 is Some n' then n' p.2
+                             else None)
               (\bigcup_(x <- domm n)
                   if n x is Some n' then pair x @: domm n'
                   else fset0).
